\documentclass{article}[12pt]
\usepackage{amsmath}

\newcommand{\pto}{\overset{P}{\to}}
\newcommand{\dto}{\overset{d}{\to}}
\newcommand{\as}{\;a.s.\;}
\newcommand{\asto}{\overset{\as}{\to}}

\title{Biostat 801 Homework 6}
\author{David Zhang}

\begin{document}
\maketitle

\section{Problem}

Let $m \geq 1$.
Then
\begin{align*}
  P[|X-Y| > 1/m]
  & \leq P[|X-X_n| + |Y-X_n| > \frac{1}{m}] \\
  & \leq P([|X-X_n| > \frac{1}{2m}] \cup [|Y-X_n| > \frac{1}{2m}]) \\
  & \leq P[|X-X_n| > \frac{1}{2m}] + P[|Y-X_n| > \frac{1}{2m}] \\
  & \to 0 \text{ as } n \to \infty.
\end{align*}
Thus $P[|X-Y| > \frac{1}{m}] = 0$.
Then
\begin{align*}
  P[X \neq Y]
  & = P[|X-Y|>0]
    = P(\bigcup_{m=1}^\infty [|X-Y| > \frac{1}{m}]) \\
  & = \lim_{m \to \infty} P[|X-Y| > \frac{1}{m}]
    = \lim_{m \to \infty} 0
    = 0
\end{align*}

\section{Problem}

\subsection{}

We have
\begin{align*}
  P[||X|-|X_n|| < \epsilon]
  & \leq P[|X - X_n| < \epsilon]
    \to 0.
\end{align*}
Thus $|X_n| \pto |X_n|$.

\subsection{}

\begin{enumerate}
\item To show: $X_n Y \pto XY$. \\
  Proof: We have
  \begin{align*}
    & P[|X_n Y - XY| > \epsilon] \\
    = & P[|X_n-X||Y| > \epsilon] \\
    = & P([|X_n-X||Y| > \epsilon] \cap  [|Y| > M]) \cup ([|X_n-X||Y| > \epsilon] \cap  [|Y| \leq M]) \\
    \leq & P[|Y| > M] + P[|X_n-X|M > \epsilon] \\
    \to & P[|Y| > M] \text{ as } n \to \infty
  \end{align*}
  Since $M \geq 1$ is arbitrary and $P[|Y| > M] \to 0$ as $M \to \infty$,
  we conclude that $\lim_{n \to \infty} P[|X_nY - XY| > \epsilon] = 0$.
\item To show: $X_n Y_n \pto X Y_n$. \\
  Proof: Following the previous arguement, we have
  \begin{align*}
    P[|X_n Y - XY| > \epsilon] \leq P[|Y_n| > M] + P[|X_n-X|M > \epsilon] 
  \end{align*}
  Since
  \[
    Y_n \pto Y \Rightarrow |Y_n| \pto |Y| \Rightarrow |Y_n| \dto |Y|,
  \]
  we have
  \[
    \lim_{n \to \infty} P[|Y_n| > M] = P[|Y| > M].
  \]
  Then
  \[
    \lim_{n \to \infty} P[|X_n Y - XY| = P[|Y| > M] \to 0
  \]
  as we let $M \to \infty$.
\item To show: $X_nY_n \pto XY$. \\
  Proof: We have
  \begin{align*}
    & P[|X_nY_n-XY| > \epsilon] \\
    \leq & P[|X_nY_n-X_nY| + |X_nY-XY| > \epsilon] \\
    \leq & P[|X_n Y_n - X_n Y| > \frac{\epsilon}{2}] + P[|X_n Y - XY| > \frac{\epsilon}{2}] \\
    \to & 0 \quad\text{as}\quad n \to \infty.
  \end{align*}
\end{enumerate}

\section{Problem}

\subsection{}
Since $X_n \asto X$,
\[
  \lim_{n \to \infty} X_n(\omega) = X(\omega) \quad \forall \omega \in A
\]
for some $A \subset \Omega$ with $P(A^C) = 0$.
Then 
\[
  \lim_{n \to \infty} |X_n(\omega)| = |X(\omega)| \quad \forall \omega \in A.
\]
Thus $|X_n| \asto |X|$.

\subsection{}
We have
\[
  \lim_{n \to \infty} X_n(\omega) = X(\omega) \quad \forall \omega \in A
\]
and
\[
  \lim_{n \to \infty} Y_n(\omega) = Y(\omega) \quad \forall \omega \in B
\]
for some $A, B \subset \Omega$ with $P(A^C) = P(B^C) = 0$.
Then
\[
  P((AB)^C) = P(A^C \cup B^C) \leq P(A^C) + P(B^C) = 0
\]
and
\[
  \lim_{n \to \infty} X_n(\omega)Y_n(\omega) = X(\omega)Y(\omega) \quad \forall \omega \in AB.
\]
Thus $X_n Y_n \asto XY$.

\end{document}
