\documentclass{article}

\usepackage{amsmath}

\newcommand{\hf}{\hat{f}}
\newcommand{\hF}{\hat{F}}
\newcommand{\Bern}{\operatorname{Bern}}
\newcommand{\ltwo}{\overset{L_2}{\to}}
\newcommand{\pto}{\overset{p}{\to}}
\newcommand{\dto}{\overset{d}{\to}}
\newcommand{\iid}{\overset{iid}{\sim}}

\title{Biostat 801 Homework 8}
\author{David Zhang}
\begin{document}
\maketitle

\section{Problem}

Let
\[
  Y_{n,i}(x) = 1_{[X_i \in (x - a_n, x+a_n]]} \iid \Bern(p_n(x))
\]
where
\[
  p_n(x) = F((x - a_n, x+a_n]).
\]
Then
\[
  p_n(x) \to 0 \quad\text{and}\quad \frac{p_n(x)}{2a_n} \to f(x)
\]
as $a_n \to 0$.
Moreover,
\begin{align*}
  E[\hf_n(x)]
  = & E \left[ \frac{\hF_n(x+a_n) - \hF_n(x-a_n)}{2a_n} \right]
  \\ = & E \left[\frac{\sum_{i=1}^n Y_{n,i}(x)}{2na_n} \right]
  \\ = & \frac{n p_n(x)}{2na_n}
  \\ = & \frac{p_n(x)}{2a_n}
         \to f(x) \quad\text{as}\quad a_n \to 0
\end{align*}

\section{Problem}

From the previous problem, we have

\begin{align*}
Var[\hf_n(x)] = & \frac{Var \sum_{i=1}^n Y_{n,i}(x)}{4n^2a_n^2} 
  \\ = & \frac{n p_n(x)(1 - p_n(x))}{4n^2a_n^2}
  \\ = & \frac{1}{2na_n}\frac{p_n(x)}{2a_n} (1 - p_n(x))
         \\ \to & 0 \cdot f(x) \cdot (1 - 0) = 0
\end{align*}
as $a_n \to 0$ and $na_n \to \infty$.

\section{Problem}
We have
\[
  E\{(\hf_n(x) - E[\hf_n(x)])^2\} = Var[\hf_n(x)] \to 0
\]
as $na_n \to \infty$, so
\[
  \hf_n(x) \ltwo E[\hf_n(x)].
\]
Moreover, since $E[\hf_n(x)] \to f(x)$,
\[
  E[\hf_n(x)] \ltwo f(x).
\]
Then by the triangular inequality,
\[
  \hf_n(x) \ltwo f(x),
\]
which implies
\[
  \hf_n(x) \pto f(x).
\]
Thus $\hf_n$ is a consistent estimator for $f$.

\section{Problem}

Let
\[
  W_{n,i}(x) = \frac{Y_{n,i}(x)}{2a_n}.
\]
Then
\begin{align*}
  \hf_n(x) = & \frac{1}{n} \sum_{i=1}^n W_{n,i}(x) = \bar{W}_n(x).
  \\ E[\hf_n(x)] = & \frac{1}{n} \sum_{i=1}^n E[W_{n,i}(x)] = E[W_{n,1}(x)] =  \frac{p_n(x)}{2a_n}
\end{align*}
and
\[
  Var[W_{n,1}(x)] = \frac{p_n(x)}{2a_n} \frac{(1-p_n(x))}{2a_n} \to
  \frac{f(x)}{2a_n}
\]
as $a_n \to 0$.  Then as $n \to \infty$ and $a_n \to 0$,
\begin{align*}
  \frac{\bar{W}_n(x) - E[W_{n,1}(x)]}{\sqrt{Var[W_{n,1}(x)] / n}}
  \to \sqrt{2na_n} \frac{\hf_n(x) - E\hf_n(x)}{\sqrt{f(x)}} 
\end{align*}
and by CLT,
\[
  \frac{\bar{W}_n(x) - E[W_{n,1}(x)]}{\sqrt{Var[W_{n,1}(x)] / n}} \dto
  N(0,1).
\]
Then by Slutsky,
\[
  \sqrt{2na_n} \frac{\hf_n(x) - E\hf_n(x)}{\sqrt{f(x)}} \dto N(0,1).
\]

\end{document}
